RState.v
@@ -14,10 +14,9 @@ Open Scope program_scope.
 
 Section RState.
 
-Variable   s   : Type.
-Variable   ist : s.
-Hypothesis P   : relation s.
-Context  `(e   : PreOrder s P).
+Variable   s : Type.
+Hypothesis P : relation s.
+Context  `(e : PreOrder s P).
 
 Record StateP (before : s) (a : Type) := {
     after  : s;
@@ -32,16 +31,18 @@ Arguments holds [before] [a] _.
 (** The [RState] monad requires that a given equivalence relation hold
     between state transitions. *)
 Inductive RState (a : Type) : Type :=
-  | St : (forall st : s, P ist st -> StateP st a) -> RState a.
+  | St : (forall st : s, StateP st a) -> RState a.
 
 Arguments St [a] _.
 
 Definition runRState {a : Type} (v : RState a)
-  : forall st : s, P ist st -> StateP st a := match v with St f => f end.
+  : forall st : s, StateP st a :=
+      match v with St f => fun st => f st end.
 
-Definition RState_fmap (a b : Type) (f : a -> b) (x : RState a) : RState b :=
-  St (fun st H =>
-        let sp := runRState x st H in
+Definition RState_fmap (a b : Type) (f : a -> b) (x : RState a)
+  : RState b :=
+  St (fun st =>
+        let sp := runRState x st in
         {| after  := after sp
          ; result := f (result sp)
          ; holds  := holds sp
@@ -52,36 +53,27 @@ Hint Unfold RState_fmap.
 Ltac RState_auto :=
   intros; simpl;
   repeat (
-    autounfold; simpl;
-    f_equal; try apply proof_irrelevance; simpl;
-    repeat match goal with
+    autounfold; unfold id, compose; simpl;
+    f_equal; try apply proof_irrelevance; auto;
+    match goal with
     | [ |- (fun _ : RState _ => _) = (fun _ : RState _ => _) ] =>
         extensionality sx
     | [ |- (fun _ : s => _) = _ ] =>
         extensionality st
-    | [ |- (fun _ : P ist _ => _) = _ ] =>
-        extensionality Hp
-    | [ st : s, Hp: P ist _,
-        sp : forall st : s, P ist st -> StateP st _ |- _ ] =>
-        repeat match goal with [ |- context [sp st ?H] ] =>
-          first [ is_var H
-                | assert (Hp = H) as Hi by (apply proof_irrelevance);
-                  rewrite <- Hi; clear Hi ]
-        end;
-        destruct (sp st); clear sp
-    | [ sx : RState _ |- _ ] =>
-        destruct sx; clear sx
-    | [ |- St _ = St _ ] =>
-        f_equal
-    end; simpl).
+    | [ st : s, sp : forall st : s, StateP st _ |- _ ] =>
+        destruct (sp st)
+    | [ sx : RState _ |- _ ] => destruct sx as [sp]
+    | [ |- St _ = St _ ] => f_equal
+    end).
 
-Global Program Instance RState_Functor : Functor RState := {
+Obligation Tactic := RState_auto.
+
+Program Instance RState_Functor : Functor RState := {
     fmap := RState_fmap
 }.
-Solve All Obligations using RState_auto.
 
 Definition RState_pure (a : Type) (x : a) : RState a :=
-  St (fun st _ =>
+  St (fun st =>
         {| after  := st
          ; result := x
          ; holds  := reflexivity st
@@ -91,10 +83,9 @@ Hint Unfold RState_pure.
 
 Definition RState_ap (a b : Type) (f : RState (a -> b)) (x : RState a)
   : RState b :=
-  St (fun st H =>
-        let spf := runRState f st H in
-        let spx := runRState x (after spf)
-                             (transitivity H (holds spf)) in
+  St (fun st =>
+        let spf := runRState f st in
+        let spx := runRState x (after spf) in
         {| after  := after spx
          ; result := (result spf) (result spx)
          ; holds  := transitivity (holds spf) (holds spx)
@@ -102,57 +93,15 @@ Definition RState_ap (a b : Type) (f : RState (a -> b)) (x : RState a)
 
 Hint Unfold RState_ap.
 
-Global Program Instance RState_Applicative : Applicative RState := {
+Program Instance RState_Applicative : Applicative RState := {
     pure := RState_pure;
     ap   := RState_ap
 }.
-Obligation 2.
-  destruct u as [su].
-  destruct v as [sv].
-  destruct w as [sw].
-  unfold RState_pure, compose.
-  unfold RState_ap. simpl.
-  f_equal.
-  extensionality st.
-  extensionality Hp. simpl.
-  assert (Hp = transitivity (x:=ist) (y:=st) (z:=st) Hp (reflexivity st))
-    by (apply proof_irrelevance).
-  rewrite <- H. clear H.
-  destruct (su st). simpl.
-  assert (transitivity (x:=ist) (y:=st) (z:=after0) Hp
-                       (transitivity (x:=st) (y:=st) (z:=after0)
-                          (reflexivity st) holds0) =
-          transitivity (x:=ist) (y:=st) (z:=after0) Hp holds0)
-    by (apply proof_irrelevance).
-  rewrite <- H. clear H.
-  destruct (sv after0). simpl.
-  assert (transitivity (x:=ist) (y:=st) (z:=after1) Hp
-                       (transitivity (x:=st) (y:=after0) (z:=after1)
-                         (transitivity (x:=st) (y:=st) (z:=after0)
-                            (reflexivity st) holds0) holds1) =
-          transitivity (x:=ist) (y:=after0) (z:=after1)
-                       (transitivity (x:=ist) (y:=st) (z:=after0) Hp
-                          (transitivity (x:=st) (y:=st) (z:=after0)
-                             (reflexivity st) holds0)) holds1)
-    by (apply proof_irrelevance).
-  rewrite <- H. clear H.
-  destruct (sw after1). simpl.
-  f_equal. apply proof_irrelevance.
-Qed.
-Obligation 4.
-  RState_auto.
-  assert (Hp = transitivity (x:=ist) (y:=st) (z:=st) Hp (reflexivity st))
-    by (apply proof_irrelevance).
-  rewrite <- H. clear H.
-  f_equal. apply proof_irrelevance.
-Qed.
-Solve All Obligations using RState_auto.
 
 Definition RState_join (a : Type) (x : RState (RState a)) : RState a :=
-  St (fun st H =>
-        let sp := runRState x st H in
-        let sp' := runRState (result sp) (after sp)
-                             (transitivity H (holds sp)) in
+  St (fun st =>
+        let sp := runRState x st in
+        let sp' := runRState (result sp) (after sp) in
         {| after  := after sp'
          ; result := result sp'
          ; holds  := transitivity (holds sp) (holds sp')
@@ -160,30 +109,12 @@ Definition RState_join (a : Type) (x : RState (RState a)) : RState a :=
 
 Hint Unfold RState_join.
 
-Global Program Instance RState_Monad : Monad RState := {
+Program Instance RState_Monad : Monad RState := {
     join := RState_join
 }.
-Obligation 1.
-  intros. autounfold. simpl.
-  extensionality sx. f_equal.
-  destruct sx as [sp]. simpl.
-  extensionality st.
-  extensionality H.
-  destruct (sp st). simpl.
-  destruct result0. simpl.
-  destruct (s0 after0). simpl.
-  assert (transitivity (x:=ist) (y:=after0) (z:=after1)
-            (transitivity (x:=ist) (y:=st) (z:=after0) H holds0) holds1 =
-          transitivity (x:=ist) (y:=st) (z:=after1) H
-            (transitivity (x:=st) (y:=after0) (z:=after1) holds0 holds1))
-    by (apply proof_irrelevance).
-  rewrite H0. clear H0.
-  f_equal. apply proof_irrelevance.
-Qed.
-Solve All Obligations using RState_auto.
 
 Definition get : RState s :=
-  St (fun st _ =>
+  St (fun st =>
         {| after  := st
          ; result := st
          ; holds  := reflexivity st
@@ -192,13 +123,12 @@ Definition get : RState s :=
 (** There cannot be a definition of [put], since we can only lawfully
     transform the state, not simply replace it.  Therefore, [modify] must be
     used in all cases where [put] would ordinarily have been. *)
-
 Definition modify (f : forall st : s, { st' : s & P st st' }) : RState unit :=
-  St (fun st _ =>
-        let (st', H') := f st in
+  St (fun st =>
+        let (st', H) := f st in
         {| after  := st'
          ; result := tt
-         ; holds  := H'
+         ; holds  := H
          |}).
 
 End RState.
